Source/DafnyRuntime/DafnyRuntimeDafny/src/toArrayOptimized.dfy
@@ -1,0 +1,92 @@
+
+include "array.dfy"
+include "frames.dfy"
+include "sequence.dfy"
+
+module {:options "/functionSyntax:4"} ToArrayOptimized {
+
+  import opened Arrays
+  import opened Frames
+  import opened MetaSeq
+  
+  method ToArrayOptimized<T>(e: Concat<T>) returns (ret: ResizableArray<T>)
+    requires e.Valid()
+    ensures ret.Valid()
+    ensures ret.Value() == e.Value()
+  {
+    var builder := new ResizableArray<T>(e.length);
+    var stack := new ResizableArray<SeqExpr<T>>(10);
+    stack.AddLast(e);
+    // assert stack.Value() == [e];
+    // LemmaConcatValueOnStackWithTip([], e);
+    // assert ConcatValueOnStack(stack.Value()) == e.Value();
+    while 0 < stack.size 
+      invariant stack.Valid()
+      // invariant PairwiseDisjoint({builder as Validatable, stack as Validatable} + (set v: Validatable <- stack.Value()))
+      invariant builder.Valid()
+      invariant fresh(builder.Repr)
+      invariant fresh(stack.Repr)
+      invariant forall e <- stack.Value() :: e.Valid()
+      invariant builder.Value() + ConcatValueOnStack(stack.Value()) == e.Value()
+      decreases if 0 < stack.size then stack.Last().Size() else 0, SizeSum(stack.Value())
+    {
+      var next: SeqExpr<T> := stack.RemoveLast();
+      if next is Concat<T> {
+        var concat := next as Concat<T>;
+        // ghost var stackBefore := stack.Value();
+        stack.AddLast(concat.right);
+        // LemmaConcatValueOnStackWithTip(stackBefore, concat.right);
+        // ghost var stackInbetween := stack.Value();
+        stack.AddLast(concat.left);
+        // LemmaConcatValueOnStackWithTip(stackInbetween, concat.left);
+      } else if next is Lazy<T> {
+        var lazy := next as Lazy<T>;
+        var boxed := lazy.exprBox.Get();
+        stack.AddLast(boxed);
+      } else {
+        var a := next.ToArray();
+        builder.Append(a);
+      }
+    }
+    return builder;
+  }
+
+  ghost function ConcatValueOnStack<T>(s: seq<SeqExpr<T>>): seq<T>
+    reads (set e <- s, o <- e.Repr :: o)
+    requires (forall e <- s :: e.Valid())
+  {
+    if |s| == 0 then
+      []
+    else
+      s[|s| - 1].Value() + ConcatValueOnStack(s[..(|s| - 1)])
+  }
+
+  lemma LemmaConcatValueOnStackWithTip<T>(s: seq<SeqExpr<T>>, x: SeqExpr<T>) 
+    requires (forall e <- s :: e.Valid())
+    requires x.Valid()
+    ensures ConcatValueOnStack(s + [x]) == x.Value() + ConcatValueOnStack(s)
+  {
+    // var valueFn := (e: SeqExpr<T>) reads e, e.Repr requires e.Valid() => e.Value();
+    // calc {
+    //   ConcatValueOnStack(s + [x]);
+    //   Seq.Flatten(Seq.Map(valueFn, Seq.Reverse(s + [x])));
+    //   { reveal Seq.Reverse(); }
+    //   Seq.Flatten(Seq.Map(valueFn, [x] + Seq.Reverse(s)));
+    //   { reveal Seq.Map(); }
+    //   Seq.Flatten([x.Value()] + Seq.Map(valueFn, Seq.Reverse(s)));
+    //   x.Value() + Seq.Flatten(Seq.Map(valueFn, Seq.Reverse(s)));
+    //   x.Value() + ConcatValueOnStack(s);
+    // }
+  }
+
+  ghost function SizeSum<T>(s: seq<SeqExpr<T>>): nat 
+    reads set e <- s, o <- e.Repr :: o
+    requires forall e <- s :: e.Valid()
+  {
+    if |s| == 0 then 
+      0 
+    else
+      var last := |s| - 1;
+      SizeSum(s[..last]) + s[last].Size()
+  }
+}
